low/Rfeatures.v
@@ -4,5 +4,45 @@
 Set Implicit Arguments.
 Require Export Reval.
 
-(* TODO *)
+
+Section Parameters.
+
+Variable globals : Globals.
+
+Let read_globals : GlobalVariable -> SExpRec_pointer := globals.
+
+Local Coercion read_globals : GlobalVariable >-> SExpRec_pointer.
+
+Variable runs : runs_type.
+
+(** * eval.c **)
+
+(** The function names of this section corresponds to the function names
+ * in the file main/eval.c. **)
+
+Definition do_set S (call op args rho : SExpRec_pointer) : result SExpRec_pointer :=
+  let wrong S := result_error S "[do_set] Wrong argument count." in
+  ifb args = R_NilValue then wrong S
+  else read%list args_, args_list := args using S in
+  ifb list_cdrval args_list = R_NilValue then wrong S
+  else read%list args_cdr_, args_cdr_list := list_cdrval args_list using S in
+  ifb list_cdrval args_cdr_list = R_NilValue then wrong S
+  else
+    read%defined lhs_ := list_carval args_list using S in
+    let symcase S :=
+      let%success rhs := runs_eval runs (list_carval args_cdr_list) rho using S in
+      let%success _ := INCREMENT_NAMED S rhs using S in
+      result_not_implemented "[do_set] TODO" in
+    match type lhs_ with
+    | StrSxp =>
+      let%success lhs_char := STRING_ELT S lhs 0 using S in
+      let%success lhs := installTrChar lhs_char using S in
+      symcase S
+    | SymSxp => symcase S
+    | LangSxp => result_not_implemented "[do_set] TODO"
+    | _ => result_error S "[do_set] Invalid left-hand side to assignment."
+    end.
+
+
+End Parameters.
 
